converted to Isar

src/HOL/IMP/Expr.thy
@@ -2,20 +2,24 @@
     ID:         $Id$
     Author:     Heiko Loetzbeyer & Robert Sandner & Tobias Nipkow, TUM
     Copyright   1994 TUM
-
-Arithmetic expressions and Boolean expressions.
-Not used in the rest of the language, but included for completeness.
 *)
 
-Expr = Datatype +
+header "Expressions"
 
-(** Arithmetic expressions **)
-types loc
-      state = "loc => nat"
-      n2n = "nat => nat"
-      n2n2n = "nat => nat => nat"
+theory Expr = Datatype:
 
-arities loc :: type
+text {*
+  Arithmetic expressions and Boolean expressions.
+  Not used in the rest of the language, but included for completeness.
+*}
+
+subsection "Arithmetic expressions"
+typedecl loc 
+
+types
+  state = "loc => nat"
+  n2n = "nat => nat"
+  n2n2n = "nat => nat => nat"
 
 datatype
   aexp = N nat
@@ -23,22 +27,24 @@ datatype
        | Op1 n2n aexp
        | Op2 n2n2n aexp aexp
 
-(** Evaluation of arithmetic expressions **)
+subsection "Evaluation of arithmetic expressions"
 consts  evala    :: "((aexp*state) * nat) set"
        "-a->"    :: "[aexp*state,nat] => bool"         (infixl 50)
 translations
     "aesig -a-> n" == "(aesig,n) : evala"
 inductive evala
-  intrs 
-    N   "(N(n),s) -a-> n"
-    X   "(X(x),s) -a-> s(x)"
-    Op1 "(e,s) -a-> n ==> (Op1 f e,s) -a-> f(n)"
-    Op2 "[| (e0,s) -a-> n0;  (e1,s)  -a-> n1 |] 
-           ==> (Op2 f e0 e1,s) -a-> f n0 n1"
+  intros 
+  N:   "(N(n),s) -a-> n"
+  X:   "(X(x),s) -a-> s(x)"
+  Op1: "(e,s) -a-> n ==> (Op1 f e,s) -a-> f(n)"
+  Op2: "[| (e0,s) -a-> n0;  (e1,s)  -a-> n1 |] 
+        ==> (Op2 f e0 e1,s) -a-> f n0 n1"
+
+lemmas [intro] = N X Op1 Op2
 
 types n2n2b = "[nat,nat] => bool"
 
-(** Boolean expressions **)
+subsection "Boolean expressions"
 
 datatype
   bexp = true
@@ -48,7 +54,7 @@ datatype
        | andi bexp bexp         (infixl 60)
        | ori  bexp bexp         (infixl 60)
 
-(** Evaluation of boolean expressions **)
+subsection "Evaluation of boolean expressions"
 consts evalb    :: "((bexp*state) * bool)set"       
        "-b->"   :: "[bexp*state,bool] => bool"         (infixl 50)
 
@@ -56,21 +62,24 @@ translations
     "besig -b-> b" == "(besig,b) : evalb"
 
 inductive evalb
- intrs (*avoid clash with ML constructors true, false*)
-    tru   "(true,s) -b-> True"
-    fls   "(false,s) -b-> False"
-    ROp   "[| (a0,s) -a-> n0; (a1,s) -a-> n1 |] 
-           ==> (ROp f a0 a1,s) -b-> f n0 n1"
-    noti  "(b,s) -b-> w ==> (noti(b),s) -b-> (~w)"
-    andi  "[| (b0,s) -b-> w0; (b1,s) -b-> w1 |] 
+  -- "avoid clash with ML constructors true, false"
+  intros
+  tru:   "(true,s) -b-> True"
+  fls:   "(false,s) -b-> False"
+  ROp:   "[| (a0,s) -a-> n0; (a1,s) -a-> n1 |] 
+          ==> (ROp f a0 a1,s) -b-> f n0 n1"
+  noti:  "(b,s) -b-> w ==> (noti(b),s) -b-> (~w)"
+  andi:  "[| (b0,s) -b-> w0; (b1,s) -b-> w1 |] 
           ==> (b0 andi b1,s) -b-> (w0 & w1)"
-    ori   "[| (b0,s) -b-> w0; (b1,s) -b-> w1 |] 
-            ==> (b0 ori b1,s) -b-> (w0 | w1)"
+  ori:   "[| (b0,s) -b-> w0; (b1,s) -b-> w1 |] 
+          ==> (b0 ori b1,s) -b-> (w0 | w1)"
 
-(** Denotational semantics of arithemtic and boolean expressions **)
+lemmas [intro] = tru fls ROp noti andi ori
+
+subsection "Denotational semantics of arithmetic and boolean expressions"
 consts
-  A     :: aexp => state => nat
-  B     :: bexp => state => bool
+  A     :: "aexp => state => nat"
+  B     :: "bexp => state => bool"
 
 primrec
   "A(N(n)) = (%s. n)"
@@ -85,6 +94,60 @@ primrec
   "B(noti(b)) = (%s. ~(B b s))"
   "B(b0 andi b1) = (%s. (B b0 s) & (B b1 s))"
   "B(b0 ori b1) = (%s. (B b0 s) | (B b1 s))"
+
+lemma [simp]: "(N(n),s) -a-> n' = (n = n')"
+  by (rule,cases set: evala) auto
+
+lemma [simp]: "(X(x),sigma) -a-> i = (i = sigma x)" 
+  by (rule,cases set: evala) auto
+
+lemma	[simp]: 
+  "(Op1 f e,sigma) -a-> i = (\<exists>n. i = f n \<and> (e,sigma) -a-> n)" 
+  by (rule,cases set: evala) auto
+
+lemma [simp]:
+  "(Op2 f a1 a2,sigma) -a-> i = 
+  (\<exists>n0 n1. i = f n0 n1 \<and> (a1, sigma) -a-> n0 \<and> (a2, sigma) -a-> n1)"
+  by (rule,cases set: evala) auto
+
+lemma [simp]: "((true,sigma) -b-> w) = (w=True)" 
+  by (rule,cases set: evalb) auto
+
+lemma [simp]:
+  "((false,sigma) -b-> w) = (w=False)" 
+  by (rule,cases set: evalb) auto
+
+lemma [simp]:
+  "((ROp f a0 a1,sigma) -b-> w) =   
+  (? m. (a0,sigma) -a-> m & (? n. (a1,sigma) -a-> n & w = f m n))" 
+  by (rule,cases set: evalb) auto
+
+lemma [simp]:  
+  "((noti(b),sigma) -b-> w) = (? x. (b,sigma) -b-> x & w = (~x))" 
+  by (rule,cases set: evalb) auto
+
+lemma [simp]:
+  "((b0 andi b1,sigma) -b-> w) =   
+  (? x. (b0,sigma) -b-> x & (? y. (b1,sigma) -b-> y & w = (x&y)))" 
+  by (rule,cases set: evalb) auto
+
+lemma [simp]:  
+  "((b0 ori b1,sigma) -b-> w) =   
+  (? x. (b0,sigma) -b-> x & (? y. (b1,sigma) -b-> y & w = (x|y)))" 
+  by (rule,cases set: evalb) auto
+
+
+lemma aexp_iff [rule_format (no_asm)]: 
+  "!n. ((a,s) -a-> n) = (A a s = n)"
+  apply (induct_tac "a")
+  apply auto
+  done
+
+lemma bexp_iff [rule_format (no_asm)]: 
+  "!w. ((b,s) -b-> w) = (B b s = w)"
+  apply (induct_tac "b")
+  apply (auto simp add: aexp_iff)
+  done
 
 end
 
