src/HOL/IMP/Hoare.thy
@@ -2,34 +2,157 @@
     ID:         $Id$
     Author:     Tobias Nipkow
     Copyright   1995 TUM
-
-Inductive definition of Hoare logic
 *)
 
-Hoare = Denotation + Inductive +
+header "Inductive Definition of Hoare Logic"
 
-types assn = state => bool
+theory Hoare = Denotation:
 
-constdefs hoare_valid :: [assn,com,assn] => bool ("|= {(1_)}/ (_)/ {(1_)}" 50)
+types assn = "state => bool"
+
+constdefs hoare_valid :: "[assn,com,assn] => bool" ("|= {(1_)}/ (_)/ {(1_)}" 50)
           "|= {P}c{Q} == !s t. (s,t) : C(c) --> P s --> Q t"
 
 consts hoare :: "(assn * com * assn) set"
-syntax "@hoare" :: [bool,com,bool] => bool ("|- ({(1_)}/ (_)/ {(1_)})" 50)
+syntax "@hoare" :: "[bool,com,bool] => bool" ("|- ({(1_)}/ (_)/ {(1_)})" 50)
 translations "|- {P}c{Q}" == "(P,c,Q) : hoare"
 
 inductive hoare
-intrs
-  skip "|- {P}SKIP{P}"
-  ass  "|- {%s. P(s[x::=a s])} x:==a {P}"
-  semi "[| |- {P}c{Q}; |- {Q}d{R} |] ==> |- {P} c;d {R}"
-  If "[| |- {%s. P s & b s}c{Q}; |- {%s. P s & ~b s}d{Q} |] ==>
-      |- {P} IF b THEN c ELSE d {Q}"
-  While "|- {%s. P s & b s} c {P} ==>
-         |- {P} WHILE b DO c {%s. P s & ~b s}"
-  conseq "[| !s. P' s --> P s; |- {P}c{Q}; !s. Q s --> Q' s |] ==>
+intros
+  skip: "|- {P}\<SKIP>{P}"
+  ass:  "|- {%s. P(s[x\<mapsto>a s])} x:==a {P}"
+  semi: "[| |- {P}c{Q}; |- {Q}d{R} |] ==> |- {P} c;d {R}"
+  If: "[| |- {%s. P s & b s}c{Q}; |- {%s. P s & ~b s}d{Q} |] ==>
+      |- {P} \<IF> b \<THEN> c \<ELSE> d {Q}"
+  While: "|- {%s. P s & b s} c {P} ==>
+         |- {P} \<WHILE> b \<DO> c {%s. P s & ~b s}"
+  conseq: "[| !s. P' s --> P s; |- {P}c{Q}; !s. Q s --> Q' s |] ==>
           |- {P'}c{Q'}"
 
-constdefs wp :: com => assn => assn
+constdefs wp :: "com => assn => assn"
           "wp c Q == (%s. !t. (s,t) : C(c) --> Q t)"
+
+(*  
+Soundness (and part of) relative completeness of Hoare rules
+wrt denotational semantics
+*)
+
+lemma hoare_conseq1: "[| !s. P' s --> P s; |- {P}c{Q} |] ==> |- {P'}c{Q}"
+apply (erule hoare.conseq)
+apply  assumption
+apply fast
+done
+
+lemma hoare_conseq2: "[| |- {P}c{Q}; !s. Q s --> Q' s |] ==> |- {P}c{Q'}"
+apply (rule hoare.conseq)
+prefer 2 apply    (assumption)
+apply fast
+apply fast
+done
+
+lemma hoare_sound: "|- {P}c{Q} ==> |= {P}c{Q}"
+apply (unfold hoare_valid_def)
+apply (erule hoare.induct)
+     apply (simp_all (no_asm_simp))
+  apply fast
+ apply fast
+apply (rule allI, rule allI, rule impI)
+apply (erule lfp_induct2)
+ apply (rule Gamma_mono)
+apply (unfold Gamma_def)
+apply fast
+done
+
+lemma wp_SKIP: "wp \<SKIP> Q = Q"
+apply (unfold wp_def)
+apply (simp (no_asm))
+done
+
+lemma wp_Ass: "wp (x:==a) Q = (%s. Q(s[x\<mapsto>a s]))"
+apply (unfold wp_def)
+apply (simp (no_asm))
+done
+
+lemma wp_Semi: "wp (c;d) Q = wp c (wp d Q)"
+apply (unfold wp_def)
+apply (simp (no_asm))
+apply (rule ext)
+apply fast
+done
+
+lemma wp_If: 
+ "wp (\<IF> b \<THEN> c \<ELSE> d) Q = (%s. (b s --> wp c Q s) &  (~b s --> wp d Q s))"
+apply (unfold wp_def)
+apply (simp (no_asm))
+apply (rule ext)
+apply fast
+done
+
+lemma wp_While_True: 
+  "b s ==> wp (\<WHILE> b \<DO> c) Q s = wp (c;\<WHILE> b \<DO> c) Q s"
+apply (unfold wp_def)
+apply (subst C_While_If)
+apply (simp (no_asm_simp))
+done
+
+lemma wp_While_False: "~b s ==> wp (\<WHILE> b \<DO> c) Q s = Q s"
+apply (unfold wp_def)
+apply (subst C_While_If)
+apply (simp (no_asm_simp))
+done
+
+declare wp_SKIP [simp] wp_Ass [simp] wp_Semi [simp] wp_If [simp] wp_While_True [simp] wp_While_False [simp]
+
+(*Not suitable for rewriting: LOOPS!*)
+lemma wp_While_if: "wp (\<WHILE> b \<DO> c) Q s = (if b s then wp (c;\<WHILE> b \<DO> c) Q s else Q s)"
+apply (simp (no_asm))
+done
+
+lemma wp_While: "wp (\<WHILE> b \<DO> c) Q s =  
+   (s : gfp(%S.{s. if b s then wp c (%s. s:S) s else Q s}))"
+apply (simp (no_asm))
+apply (rule iffI)
+ apply (rule weak_coinduct)
+  apply (erule CollectI)
+ apply safe
+  apply (rotate_tac -1)
+  apply simp
+ apply (rotate_tac -1)
+ apply simp
+apply (simp add: wp_def Gamma_def)
+apply (intro strip)
+apply (rule mp)
+ prefer 2 apply (assumption)
+apply (erule lfp_induct2)
+apply (fast intro!: monoI)
+apply (subst gfp_unfold)
+ apply (fast intro!: monoI)
+apply fast
+done
+
+declare C_while [simp del]
+
+declare hoare.skip [intro!] hoare.ass [intro!] hoare.semi [intro!] hoare.If [intro!]
+
+lemma wp_is_pre [rule_format (no_asm)]: "!Q. |- {wp c Q} c {Q}"
+apply (induct_tac "c")
+    apply (simp_all (no_asm))
+    apply fast+
+ apply (blast intro: hoare_conseq1)
+apply safe
+apply (rule hoare_conseq2)
+ apply (rule hoare.While)
+ apply (rule hoare_conseq1)
+  prefer 2 apply (fast)
+  apply safe
+ apply (rotate_tac -1, simp)
+apply (rotate_tac -1, simp)
+done
+
+lemma hoare_relative_complete: "|= {P}c{Q} ==> |- {P}c{Q}"
+apply (rule hoare_conseq1 [OF _ wp_is_pre])
+apply (unfold hoare_valid_def wp_def)
+apply fast
+done
 
 end
