src/HOL/IMP/Natural.thy
@@ -1,45 +1,283 @@
-(*  Title:      HOL/IMP/Natural.thy
-    ID:         $Id$
-    Author:     Tobias Nipkow & Robert Sandner, TUM
-    Copyright   1996 TUM
-
-Natural semantics of commands
+(*  Title:        HOL/IMP/Natural.thy
+    ID:           $Id$
+    Author:       Tobias Nipkow & Robert Sandner, TUM
+    Isar Version: Gerwin Klein, 2001
+    Copyright     1996 TUM
 *)
 
-Natural = Com + Inductive +
+header "Natural Semantics of Commands"
 
-(** Execution of commands **)
-consts  evalc    :: "(com*state*state)set"
-        "@evalc" :: [com,state,state] => bool ("<_,_>/ -c-> _" [0,0,50] 50)
+theory Natural = Com:
 
-translations  "<ce,sig> -c-> s" == "(ce,sig,s) : evalc"
+subsection "Execution of commands"
 
-consts
-  update  :: "('a => 'b) => 'a => 'b => ('a => 'b)"
-           ("_/[_/::=/_]" [900,0,0] 900)
-(* update is NOT defined, only declared!
-   Thus the whole theory is independent of its meaning!
-   If the definition (update == fun_upd) is included, proofs break.
-*)
+consts  evalc  :: "(com \<times> state \<times> state) set" 
+        "@evalc" :: "[com,state,state] \<Rightarrow> bool" ("<_,_>/ -c-> _" [0,0,60] 60)
 
+syntax (xsymbols)
+  "@evalc" :: "[com,state,state] \<Rightarrow> bool" ("\<langle>_,_\<rangle>/ \<longrightarrow>\<^sub>c _" [0,0,60] 60)
+
+text {*
+  We write @{text "\<langle>c,s\<rangle> \<longrightarrow>\<^sub>c s'"} for \emph{Statement @{text c}, started 
+  in state @{text s}, terminates in state @{text s'}}. Formally,
+  @{text "\<langle>c,s\<rangle> \<longrightarrow>\<^sub>c s'"} is just another form of saying \emph{the tuple
+  @{text "(c,s,s')"} is part of the relation @{text evalc}}:
+*}
+translations  "\<langle>c,s\<rangle> \<longrightarrow>\<^sub>c s'" == "(c,s,s') \<in> evalc"
+
+constdefs
+  update :: "('a \<Rightarrow> 'b) \<Rightarrow> 'a \<Rightarrow> 'b \<Rightarrow> ('a \<Rightarrow> 'b)" ("_/[_ ::= /_]" [900,0,0] 900)
+  "update == fun_upd"
+
+syntax (xsymbols)
+  update :: "('a \<Rightarrow> 'b) \<Rightarrow> 'a \<Rightarrow> 'b \<Rightarrow> ('a \<Rightarrow> 'b)" ("_/[_ \<mapsto> /_]" [900,0,0] 900)
+
+text {*
+  The big-step execution relation @{text evalc} is defined inductively:
+*}
 inductive evalc
-  intrs
-    Skip    "<SKIP,s> -c-> s"
+  intros 
+  Skip:    "\<langle>\<SKIP>,s\<rangle> \<longrightarrow>\<^sub>c s"
+  Assign:  "\<langle>x :== a,s\<rangle> \<longrightarrow>\<^sub>c s[x\<mapsto>a s]"
 
-    Assign  "<x :== a,s> -c-> s[x::=a s]"
+  Semi:    "\<langle>c0,s\<rangle> \<longrightarrow>\<^sub>c s'' \<Longrightarrow> \<langle>c1,s''\<rangle> \<longrightarrow>\<^sub>c s' \<Longrightarrow> \<langle>c0; c1, s\<rangle> \<longrightarrow>\<^sub>c s'"
 
-    Semi    "[| <c0,s> -c-> s2; <c1,s2> -c-> s1 |] 
-            ==> <c0 ; c1, s> -c-> s1"
+  IfTrue:  "b s \<Longrightarrow> \<langle>c0,s\<rangle> \<longrightarrow>\<^sub>c s' \<Longrightarrow> \<langle>\<IF> b \<THEN> c0 \<ELSE> c1, s\<rangle> \<longrightarrow>\<^sub>c s'"
+  IfFalse: "\<not>b s \<Longrightarrow> \<langle>c1,s\<rangle> \<longrightarrow>\<^sub>c s' \<Longrightarrow> \<langle>\<IF> b \<THEN> c0 \<ELSE> c1, s\<rangle> \<longrightarrow>\<^sub>c s'"
 
-    IfTrue "[| b s; <c0,s> -c-> s1 |] 
-            ==> <IF b THEN c0 ELSE c1, s> -c-> s1"
+  WhileFalse: "\<not>b s \<Longrightarrow> \<langle>\<WHILE> b \<DO> c,s\<rangle> \<longrightarrow>\<^sub>c s"
+  WhileTrue:  "b s \<Longrightarrow> \<langle>c,s\<rangle> \<longrightarrow>\<^sub>c s'' \<Longrightarrow> \<langle>\<WHILE> b \<DO> c, s''\<rangle> \<longrightarrow>\<^sub>c s'  
+               \<Longrightarrow> \<langle>\<WHILE> b \<DO> c, s\<rangle> \<longrightarrow>\<^sub>c s'"
 
-    IfFalse "[| ~b s; <c1,s> -c-> s1 |] 
-             ==> <IF b THEN c0 ELSE c1, s> -c-> s1"
+lemmas evalc.intros [intro] -- "use those rules in automatic proofs"
 
-    WhileFalse "~b s ==> <WHILE b DO c,s> -c-> s"
+text {*
+The induction principle induced by this definition looks like this:
 
-    WhileTrue  "[| b s;  <c,s> -c-> s2;  <WHILE b DO c, s2> -c-> s1 |] 
-               ==> <WHILE b DO c, s> -c-> s1"
+@{thm [display] evalc.induct [no_vars]}
+
+
+(@{text "\<And>"} and @{text "\<Longrightarrow>"} are Isabelle's 
+  meta symbols for @{text "\<forall>"} and @{text "\<longrightarrow>"})
+*}
+
+
+text {*
+  The rules of @{text evalc} are syntax directed, i.e.~for each
+  syntactic category there is always only one rule applicable. That
+  means we can use the rules in both directions. The proofs for this
+  are all the same: one direction is trivial, the other one is shown
+  by using the @{text evalc} rules backwards: 
+*}
+lemma skip: 
+  "\<langle>\<SKIP>,s\<rangle> \<longrightarrow>\<^sub>c s' = (s' = s)"
+  by (rule, erule evalc.elims) auto
+
+lemma assign: 
+  "\<langle>x :== a,s\<rangle> \<longrightarrow>\<^sub>c s' = (s' = s[x\<mapsto>a s])" 
+  by (rule, erule evalc.elims) auto
+
+lemma semi: 
+  "\<langle>c0; c1, s\<rangle> \<longrightarrow>\<^sub>c s' = (\<exists>s''. \<langle>c0,s\<rangle> \<longrightarrow>\<^sub>c s'' \<and> \<langle>c1,s''\<rangle> \<longrightarrow>\<^sub>c s')"
+  by (rule, erule evalc.elims) auto
+
+lemma ifTrue: 
+  "b s \<Longrightarrow> \<langle>\<IF> b \<THEN> c0 \<ELSE> c1, s\<rangle> \<longrightarrow>\<^sub>c s' = \<langle>c0,s\<rangle> \<longrightarrow>\<^sub>c s'" 
+  by (rule, erule evalc.elims) auto
+
+lemma ifFalse: 
+  "\<not>b s \<Longrightarrow> \<langle>\<IF> b \<THEN> c0 \<ELSE> c1, s\<rangle> \<longrightarrow>\<^sub>c s' = \<langle>c1,s\<rangle> \<longrightarrow>\<^sub>c s'"
+  by (rule, erule evalc.elims) auto
+
+lemma whileFalse: 
+  "\<not> b s \<Longrightarrow> \<langle>\<WHILE> b \<DO> c,s\<rangle> \<longrightarrow>\<^sub>c s' = (s' = s)"
+  by (rule, erule evalc.elims) auto  
+
+lemma whileTrue: 
+  "b s \<Longrightarrow> 
+  \<langle>\<WHILE> b \<DO> c, s\<rangle> \<longrightarrow>\<^sub>c s' = 
+  (\<exists>s''. \<langle>c,s\<rangle> \<longrightarrow>\<^sub>c s'' \<and> \<langle>\<WHILE> b \<DO> c, s''\<rangle> \<longrightarrow>\<^sub>c s')"
+  by (rule, erule evalc.elims) auto
+
+text "Again, Isabelle may use these rules in automatic proofs:"
+lemmas evalc_cases [simp] = skip assign ifTrue ifFalse whileFalse semi whileTrue
+
+subsection "Equivalence of statements"
+
+text {*
+  We call two statements @{text c} and @{text c'} equivalent wrt.~the
+  big-step semantics when \emph{@{text c} started in @{text s} terminates
+  in @{text s'} iff @{text c'} started in the same @{text s} also terminates
+  in the same @{text s'}}. Formally:
+*} 
+constdefs
+  equiv_c :: "com \<Rightarrow> com \<Rightarrow> bool" ("_ \<sim> _")
+  "c \<sim> c' \<equiv> \<forall>s s'. \<langle>c, s\<rangle> \<longrightarrow>\<^sub>c s' = \<langle>c', s\<rangle> \<longrightarrow>\<^sub>c s'"
+
+text {*
+  Proof rules telling Isabelle to unfold the definition
+  if there is something to be proved about equivalent
+  statements: *} 
+lemma equivI [intro!]:
+  "(\<And>s s'. \<langle>c, s\<rangle> \<longrightarrow>\<^sub>c s' = \<langle>c', s\<rangle> \<longrightarrow>\<^sub>c s') \<Longrightarrow> c \<sim> c'"
+  by (unfold equiv_c_def) blast
+
+lemma equivD1:
+  "c \<sim> c' \<Longrightarrow> \<langle>c, s\<rangle> \<longrightarrow>\<^sub>c s' \<Longrightarrow> \<langle>c', s\<rangle> \<longrightarrow>\<^sub>c s'"
+  by (unfold equiv_c_def) blast
+
+lemma equivD2:
+  "c \<sim> c' \<Longrightarrow> \<langle>c', s\<rangle> \<longrightarrow>\<^sub>c s' \<Longrightarrow> \<langle>c, s\<rangle> \<longrightarrow>\<^sub>c s'"
+  by (unfold equiv_c_def) blast
+
+text {*
+  As an example, we show that loop unfolding is an equivalence
+  transformation on programs:
+*}
+lemma unfold_while:
+  "(\<WHILE> b \<DO> c) \<sim> (\<IF> b \<THEN> c; \<WHILE> b \<DO> c \<ELSE> \<SKIP>)" (is "?w \<sim> ?if")
+proof -
+  -- "to show the equivalence, we look at the derivation tree for"
+  -- "each side and from that construct a derivation tree for the other side"  
+  { fix s s' assume w: "\<langle>?w, s\<rangle> \<longrightarrow>\<^sub>c s'"
+    -- "as a first thing we note that, if @{text b} is @{text False} in state @{text s},"
+    -- "then both statements do nothing:"
+    hence "\<not>b s \<Longrightarrow> s = s'" by simp
+    hence "\<not>b s \<Longrightarrow> \<langle>?if, s\<rangle> \<longrightarrow>\<^sub>c s'" by simp
+    moreover
+    -- "on the other hand, if @{text b} is @{text True} in state @{text s},"
+    -- {* then only the @{text WhileTrue} rule can have been used to derive @{text "\<langle>?w, s\<rangle> \<longrightarrow>\<^sub>c s'"} *}
+    { assume b: "b s"
+      with w obtain s'' where
+        "\<langle>c, s\<rangle> \<longrightarrow>\<^sub>c s''" and "\<langle>?w, s''\<rangle> \<longrightarrow>\<^sub>c s'" by (cases set: evalc) auto
+      -- "now we can build a derivation tree for the @{text \<IF>}"
+      -- "first, the body of the True-branch:"
+      hence "\<langle>c; ?w, s\<rangle> \<longrightarrow>\<^sub>c s'" by (rule Semi)
+      -- "then the whole @{text \<IF>}"
+      with b have "\<langle>?if, s\<rangle> \<longrightarrow>\<^sub>c s'" by (rule IfTrue)
+    }
+    ultimately 
+    -- "both cases together give us what we want:"      
+    have "\<langle>?if, s\<rangle> \<longrightarrow>\<^sub>c s'" by blast
+  }
+  moreover
+  -- "now the other direction:"
+  { fix s s' assume if: "\<langle>?if, s\<rangle> \<longrightarrow>\<^sub>c s'"
+    -- "again, if @{text b} is @{text False} in state @{text s}, then the False-branch"
+    -- "of the @{text \<IF>} is executed, and both statements do nothing:"
+    hence "\<not>b s \<Longrightarrow> s = s'" by simp
+    hence "\<not>b s \<Longrightarrow> \<langle>?w, s\<rangle> \<longrightarrow>\<^sub>c s'" by simp
+    moreover
+    -- "on the other hand, if @{text b} is @{text True} in state @{text s},"
+    -- {* then this time only the @{text IfTrue} rule can have be used *}
+    { assume b: "b s"
+      with if have "\<langle>c; ?w, s\<rangle> \<longrightarrow>\<^sub>c s'" by (cases set: evalc) auto
+      -- "and for this, only the Semi-rule is applicable:"
+      then obtain s'' where
+        "\<langle>c, s\<rangle> \<longrightarrow>\<^sub>c s''" and "\<langle>?w, s''\<rangle> \<longrightarrow>\<^sub>c s'" by (cases set: evalc) auto
+      -- "with this information, we can build a derivation tree for the @{text \<WHILE>}"
+      with b
+      have "\<langle>?w, s\<rangle> \<longrightarrow>\<^sub>c s'" by (rule WhileTrue) 
+    }
+    ultimately 
+    -- "both cases together again give us what we want:"
+    have "\<langle>?w, s\<rangle> \<longrightarrow>\<^sub>c s'" by blast
+  }
+  ultimately
+  show ?thesis by blast
+qed
+
+
+subsection "Execution is deterministic"
+
+text {*
+The following proof presents all the details:
+*}
+theorem com_det: "\<langle>c,s\<rangle> \<longrightarrow>\<^sub>c t \<and> \<langle>c,s\<rangle> \<longrightarrow>\<^sub>c u \<longrightarrow> u=t"
+proof clarify -- "transform the goal into canonical form"
+  assume "\<langle>c,s\<rangle> \<longrightarrow>\<^sub>c t"
+  thus "\<And>u. \<langle>c,s\<rangle> \<longrightarrow>\<^sub>c u \<Longrightarrow> u=t" 
+  proof (induct set: evalc)
+    fix s u assume "\<langle>\<SKIP>,s\<rangle> \<longrightarrow>\<^sub>c u"
+    thus "u = s" by simp
+  next
+    fix a s x u assume "\<langle>x :== a,s\<rangle> \<longrightarrow>\<^sub>c u"
+    thus "u = s[x \<mapsto> a s]" by simp      
+  next
+    fix c0 c1 s s1 s2 u
+    assume IH0: "\<And>u. \<langle>c0,s\<rangle> \<longrightarrow>\<^sub>c u \<Longrightarrow> u = s2"
+    assume IH1: "\<And>u. \<langle>c1,s2\<rangle> \<longrightarrow>\<^sub>c u \<Longrightarrow> u = s1"
+
+    assume "\<langle>c0;c1, s\<rangle> \<longrightarrow>\<^sub>c u"
+    then obtain s' where
+      c0: "\<langle>c0,s\<rangle> \<longrightarrow>\<^sub>c s'" and
+      c1: "\<langle>c1,s'\<rangle> \<longrightarrow>\<^sub>c u" 
+      by auto
+
+    from c0 IH0 have "s'=s2" by blast
+    with c1 IH1 show "u=s1" by blast
+  next
+    fix b c0 c1 s s1 u
+    assume IH: "\<And>u. \<langle>c0,s\<rangle> \<longrightarrow>\<^sub>c u \<Longrightarrow> u = s1" 
+
+    assume "b s" and "\<langle>\<IF> b \<THEN> c0 \<ELSE> c1,s\<rangle> \<longrightarrow>\<^sub>c u"
+    hence "\<langle>c0, s\<rangle> \<longrightarrow>\<^sub>c u" by simp
+    with IH show "u = s1" by blast
+  next
+    fix b c0 c1 s s1 u
+    assume IH: "\<And>u. \<langle>c1,s\<rangle> \<longrightarrow>\<^sub>c u \<Longrightarrow> u = s1" 
+
+    assume "\<not>b s" and "\<langle>\<IF> b \<THEN> c0 \<ELSE> c1,s\<rangle> \<longrightarrow>\<^sub>c u"
+    hence "\<langle>c1, s\<rangle> \<longrightarrow>\<^sub>c u" by simp
+    with IH show "u = s1" by blast
+  next
+    fix b c s u
+    assume "\<not>b s" and "\<langle>\<WHILE> b \<DO> c,s\<rangle> \<longrightarrow>\<^sub>c u"
+    thus "u = s" by simp
+  next
+    fix b c s s1 s2 u
+    assume "IH\<^sub>c": "\<And>u. \<langle>c,s\<rangle> \<longrightarrow>\<^sub>c u \<Longrightarrow> u = s2"
+    assume "IH\<^sub>w": "\<And>u. \<langle>\<WHILE> b \<DO> c,s2\<rangle> \<longrightarrow>\<^sub>c u \<Longrightarrow> u = s1"
+    
+    assume "b s" and "\<langle>\<WHILE> b \<DO> c,s\<rangle> \<longrightarrow>\<^sub>c u"
+    then obtain s' where
+      c: "\<langle>c,s\<rangle> \<longrightarrow>\<^sub>c s'" and
+      w: "\<langle>\<WHILE> b \<DO> c,s'\<rangle> \<longrightarrow>\<^sub>c u" 
+      by auto
+    
+    from c "IH\<^sub>c" have "s' = s2" by blast
+    with w "IH\<^sub>w" show "u = s1" by blast
+  qed
+qed
+
+
+text {*
+  This is the proof as you might present it in a lecture. The remaining
+  cases are simple enough to be proved automatically: 
+*} 
+theorem "\<langle>c,s\<rangle> \<longrightarrow>\<^sub>c t \<and> \<langle>c,s\<rangle> \<longrightarrow>\<^sub>c u \<longrightarrow> u=t" 
+proof clarify
+  assume "\<langle>c,s\<rangle> \<longrightarrow>\<^sub>c t"
+  thus "\<And>u. \<langle>c,s\<rangle> \<longrightarrow>\<^sub>c u \<Longrightarrow> u=t" 
+  proof (induct set: evalc)
+    -- "the simple @{text \<SKIP>} case for demonstration:"
+    fix s u assume "\<langle>\<SKIP>,s\<rangle> \<longrightarrow>\<^sub>c u"
+    thus "u = s" by simp
+  next
+    -- "and the only really interesting case, @{text \<WHILE>}:"
+    fix b c s s1 s2 u
+    assume "IH\<^sub>c": "\<And>u. \<langle>c,s\<rangle> \<longrightarrow>\<^sub>c u \<Longrightarrow> u = s2"
+    assume "IH\<^sub>w": "\<And>u. \<langle>\<WHILE> b \<DO> c,s2\<rangle> \<longrightarrow>\<^sub>c u \<Longrightarrow> u = s1"
+    
+    assume "b s" and "\<langle>\<WHILE> b \<DO> c,s\<rangle> \<longrightarrow>\<^sub>c u"
+    then obtain s' where
+      c: "\<langle>c,s\<rangle> \<longrightarrow>\<^sub>c s'" and
+      w: "\<langle>\<WHILE> b \<DO> c,s'\<rangle> \<longrightarrow>\<^sub>c u"
+      by auto
+    
+    from c "IH\<^sub>c" have "s' = s2" by blast
+    with w "IH\<^sub>w" show "u = s1" by blast
+  qed (best dest: evalc_cases [THEN iffD1])+ -- "prove the rest automatically"
+qed
 
 end
