src/HOL/IMP/Transition.thy
@@ -1,45 +1,686 @@
-(*  Title:      HOL/IMP/Transition.thy
-    ID:         $Id$
-    Author:     Tobias Nipkow & Robert Sandner, TUM
-    Copyright   1996 TUM
-
-Transition semantics of commands
+(*  Title:        HOL/IMP/Transition.thy
+    ID:           $Id$
+    Author:       Tobias Nipkow & Robert Sandner, TUM
+    Isar Version: Gerwin Klein, 2001
+    Copyright     1996 TUM
 *)
 
-Transition = Natural +
+header "Transition Semantics of Commands"
 
-consts  evalc1    :: "((com*state)*(com*state))set"
+theory Transition = Natural:
 
+subsection "The transition relation"
+
+text {*
+  We formalize the transition semantics as in \cite{Nielson}. This
+  makes some of the rules a bit more intuitive, but also requires
+  some more (internal) formal overhead.
+  
+  Since configurations that have terminated are written without 
+  a statement, the transition relation is not 
+  @{typ "((com \<times> state) \<times> (com \<times> state)) set"}
+  but instead:
+*}
+consts evalc1 :: "((com option \<times> state) \<times> (com option \<times> state)) set"
+
+text {*
+  Some syntactic sugar that we will use to hide the 
+  @{text option} part in configurations:
+*}
 syntax
-        "@evalc1" :: "[(com*state),(com*state)] => bool"
-                                ("_ -1-> _" [81,81] 100)
-        "@evalcn" :: "[(com*state),nat,(com*state)] => bool"
-                                ("_ -_-> _" [81,81] 100)
-        "@evalc*" :: "[(com*state),(com*state)] => bool"
-                                ("_ -*-> _" [81,81] 100)
+  "@angle" :: "[com, state] \<Rightarrow> com option \<times> state" ("<_,_>")
+  "@angle2" :: "state \<Rightarrow> com option \<times> state" ("<_>")
+
+syntax (xsymbols)
+  "@angle" :: "[com, state] \<Rightarrow> com option \<times> state" ("\<langle>_,_\<rangle>")
+  "@angle2" :: "state \<Rightarrow> com option \<times> state" ("\<langle>_\<rangle>")
 
 translations
-  "cs0 -1-> cs1"	== "(cs0,cs1) : evalc1"
-  "cs0 -1-> (c1,s1)"	== "(cs0,c1,s1) : evalc1"
+  "\<langle>c,s\<rangle>" == "(Some c, s)"
+  "\<langle>s\<rangle>" == "(None, s)"
 
-  "cs0 -n-> cs1" 	== "(cs0,cs1) : evalc1^n"
-  "cs0 -n-> (c1,s1)" 	== "(cs0,c1,s1) : evalc1^n"
+text {*
+  More syntactic sugar for the transition relation, and its
+  iteration.
+*}
+syntax
+  "@evalc1" :: "[(com option\<times>state),(com option\<times>state)] \<Rightarrow> bool"
+    ("_ -1-> _" [81,81] 100)
+  "@evalcn" :: "[(com option\<times>state),nat,(com option\<times>state)] \<Rightarrow> bool"
+    ("_ -_-> _" [81,81] 100)
+  "@evalc*" :: "[(com option\<times>state),(com option\<times>state)] \<Rightarrow> bool"
+    ("_ -*-> _" [81,81] 100)
 
-  "cs0 -*-> cs1" 	== "(cs0,cs1) : evalc1^*"
-  "cs0 -*-> (c1,s1)" 	== "(cs0,c1,s1) : evalc1^*"
+syntax (xsymbols)
+  "@evalc1" :: "[(com option\<times>state),(com option\<times>state)] \<Rightarrow> bool"
+    ("_ \<longrightarrow>\<^sub>1 _" [81,81] 100)
+  "@evalcn" :: "[(com option\<times>state),nat,(com option\<times>state)] \<Rightarrow> bool"
+    ("_ -_\<rightarrow>\<^sub>1 _" [81,81] 100)
+  "@evalc*" :: "[(com option\<times>state),(com option\<times>state)] \<Rightarrow> bool"
+    ("_ \<longrightarrow>\<^sub>1\<^sup>* _" [81,81] 100)
 
+translations
+  "cs \<longrightarrow>\<^sub>1 cs'" == "(cs,cs') \<in> evalc1"
+  "cs -n\<rightarrow>\<^sub>1 cs'" == "(cs,cs') \<in> evalc1^n" 
+  "cs \<longrightarrow>\<^sub>1\<^sup>* cs'" == "(cs,cs') \<in> evalc1^*" 
 
+  -- {* Isabelle converts @{text "(cs0,(c1,s1))"} to @{term "(cs0,c1,s1)"}, 
+        so we also include: *}
+  "cs0 \<longrightarrow>\<^sub>1 (c1,s1)" == "(cs0,c1,s1) \<in> evalc1"   
+  "cs0 -n\<rightarrow>\<^sub>1 (c1,s1)" == "(cs0,c1,s1) \<in> evalc1^n"
+  "cs0 \<longrightarrow>\<^sub>1\<^sup>* (c1,s1)" == "(cs0,c1,s1) \<in> evalc1^*" 
+
+text {*
+  Now, finally, we are set to write down the rules for our small step semantics:
+*}
 inductive evalc1
-  intrs
-    Assign "(x :== a,s) -1-> (SKIP,s[x ::= a s])"
+  intros
+  Skip:    "\<langle>\<SKIP>, s\<rangle> \<longrightarrow>\<^sub>1 \<langle>s\<rangle>"  
+  Assign:  "\<langle>x :== a, s\<rangle> \<longrightarrow>\<^sub>1 \<langle>s[x \<mapsto> a s]\<rangle>"
 
-    Semi1   "(SKIP;c,s) -1-> (c,s)"     
-    Semi2   "(c0,s) -1-> (c2,s1) ==> (c0;c1,s) -1-> (c2;c1,s1)"
+  Semi1:   "\<langle>c0,s\<rangle> \<longrightarrow>\<^sub>1 \<langle>s'\<rangle> \<Longrightarrow> \<langle>c0;c1,s\<rangle> \<longrightarrow>\<^sub>1 \<langle>c1,s'\<rangle>"
+  Semi2:   "\<langle>c0,s\<rangle> \<longrightarrow>\<^sub>1 \<langle>c0',s'\<rangle> \<Longrightarrow> \<langle>c0;c1,s\<rangle> \<longrightarrow>\<^sub>1 \<langle>c0';c1,s'\<rangle>"
 
-    IfTrue "b s ==> (IF b THEN c1 ELSE c2,s) -1-> (c1,s)"
-    IfFalse "~b s ==> (IF b THEN c1 ELSE c2,s) -1-> (c2,s)"
+  IfTrue:  "b s \<Longrightarrow> \<langle>\<IF> b \<THEN> c1 \<ELSE> c2,s\<rangle> \<longrightarrow>\<^sub>1 \<langle>c1,s\<rangle>"
+  IfFalse: "\<not>b s \<Longrightarrow> \<langle>\<IF> b \<THEN> c1 \<ELSE> c2,s\<rangle> \<longrightarrow>\<^sub>1 \<langle>c2,s\<rangle>"
 
-    WhileFalse "~b s ==> (WHILE b DO c,s) -1-> (SKIP,s)"
-    WhileTrue "b s ==> (WHILE b DO c,s) -1-> (c;WHILE b DO c,s)"
+  While:   "\<langle>\<WHILE> b \<DO> c,s\<rangle> \<longrightarrow>\<^sub>1 \<langle>\<IF> b \<THEN> c; \<WHILE> b \<DO> c \<ELSE> \<SKIP>,s\<rangle>"
+
+lemmas [intro] = evalc1.intros -- "again, use these rules in automatic proofs"
+
+(*<*)
+(* fixme: move to Relation_Power.thy *)
+lemma rel_pow_Suc_E2 [elim!]:
+  "[| (x, z) \<in> R ^ Suc n; !!y. [| (x, y) \<in> R; (y, z) \<in> R ^ n |] ==> P |] ==> P"
+  by (drule rel_pow_Suc_D2) blast
+
+lemma rtrancl_imp_rel_pow: "p \<in> R^* \<Longrightarrow> \<exists>n. p \<in> R^n"
+proof -
+  assume "p \<in> R\<^sup>*"
+  moreover obtain x y where p: "p = (x,y)" by (cases p)
+  ultimately have "(x,y) \<in> R\<^sup>*" by hypsubst
+  hence "\<exists>n. (x,y) \<in> R^n"
+  proof induct
+    fix a have "(a,a) \<in> R^0" by simp
+    thus "\<exists>n. (a,a) \<in> R ^ n" ..
+  next
+    fix a b c assume "\<exists>n. (a,b) \<in> R ^ n"
+    then obtain n where "(a,b) \<in> R^n" ..
+    moreover assume "(b,c) \<in> R"
+    ultimately have "(a,c) \<in> R^(Suc n)" by auto
+    thus "\<exists>n. (a,c) \<in> R^n" ..
+  qed
+  with p show ?thesis by hypsubst
+qed  
+(*>*)    
+text {*
+  As for the big step semantics you can read these rules in a 
+  syntax directed way:
+*}
+lemma SKIP_1: "\<langle>\<SKIP>, s\<rangle> \<longrightarrow>\<^sub>1 y = (y = \<langle>s\<rangle>)" 
+  by (rule, cases set: evalc1, auto)      
+
+lemma Assign_1: "\<langle>x :== a, s\<rangle> \<longrightarrow>\<^sub>1 y = (y = \<langle>s[x \<mapsto> a s]\<rangle>)"
+  by (rule, cases set: evalc1, auto)
+
+lemma Cond_1: 
+  "\<langle>\<IF> b \<THEN> c1 \<ELSE> c2, s\<rangle> \<longrightarrow>\<^sub>1 y = ((b s \<longrightarrow> y = \<langle>c1, s\<rangle>) \<and> (\<not>b s \<longrightarrow> y = \<langle>c2, s\<rangle>))"
+  by (rule, cases set: evalc1, auto)
+
+lemma While_1: "\<langle>\<WHILE> b \<DO> c, s\<rangle> \<longrightarrow>\<^sub>1 y = (y = \<langle>\<IF> b \<THEN> c; \<WHILE> b \<DO> c \<ELSE> \<SKIP>, s\<rangle>)"
+  by (rule, cases set: evalc1, auto)
+
+lemmas [simp] = SKIP_1 Assign_1 Cond_1 While_1
+
+
+subsection "Examples"
+
+lemma 
+  "s x = 0 \<Longrightarrow> \<langle>\<WHILE> \<lambda>s. s x \<noteq> 1 \<DO> x:== \<lambda>s. s x+1, s\<rangle> \<longrightarrow>\<^sub>1\<^sup>* \<langle>s[x \<mapsto> 1]\<rangle>"
+  (is "_ \<Longrightarrow> \<langle>?w, _\<rangle> \<longrightarrow>\<^sub>1\<^sup>* _")
+proof -
+  let ?x  = "x:== \<lambda>s. s x+1"
+  let ?if = "\<IF> \<lambda>s. s x \<noteq> 1 \<THEN> ?x; ?w \<ELSE> \<SKIP>"
+  assume [simp]: "s x = 0"
+  have "\<langle>?w, s\<rangle> \<longrightarrow>\<^sub>1  \<langle>?if, s\<rangle>" ..
+  also have "\<langle>?if, s\<rangle> \<longrightarrow>\<^sub>1 \<langle>?x; ?w, s\<rangle>" by simp 
+  also have "\<langle>?x; ?w, s\<rangle> \<longrightarrow>\<^sub>1 \<langle>?w, s[x \<mapsto> 1]\<rangle>" by (rule Semi1, simp)
+  also have "\<langle>?w, s[x \<mapsto> 1]\<rangle> \<longrightarrow>\<^sub>1 \<langle>?if, s[x \<mapsto> 1]\<rangle>" ..
+  also have "\<langle>?if, s[x \<mapsto> 1]\<rangle> \<longrightarrow>\<^sub>1 \<langle>\<SKIP>, s[x \<mapsto> 1]\<rangle>" by (simp add: update_def)
+  also have "\<langle>\<SKIP>, s[x \<mapsto> 1]\<rangle> \<longrightarrow>\<^sub>1 \<langle>s[x \<mapsto> 1]\<rangle>" ..
+  finally show ?thesis ..
+qed
+
+lemma 
+  "s x = 2 \<Longrightarrow> \<langle>\<WHILE> \<lambda>s. s x \<noteq> 1 \<DO> x:== \<lambda>s. s x+1, s\<rangle> \<longrightarrow>\<^sub>1\<^sup>* s'"
+  (is "_ \<Longrightarrow> \<langle>?w, _\<rangle> \<longrightarrow>\<^sub>1\<^sup>* s'")
+proof -
+  let ?c = "x:== \<lambda>s. s x+1"
+  let ?if = "\<IF> \<lambda>s. s x \<noteq> 1 \<THEN> ?c; ?w \<ELSE> \<SKIP>"  
+  assume [simp]: "s x = 2"
+  note update_def [simp]
+  have "\<langle>?w, s\<rangle> \<longrightarrow>\<^sub>1  \<langle>?if, s\<rangle>" ..
+  also have "\<langle>?if, s\<rangle> \<longrightarrow>\<^sub>1 \<langle>?c; ?w, s\<rangle>" by simp
+  also have "\<langle>?c; ?w, s\<rangle> \<longrightarrow>\<^sub>1 \<langle>?w, s[x \<mapsto> 3]\<rangle>" by (rule Semi1, simp)
+  also have "\<langle>?w, s[x \<mapsto> 3]\<rangle> \<longrightarrow>\<^sub>1 \<langle>?if, s[x \<mapsto> 3]\<rangle>" ..
+  also have "\<langle>?if, s[x \<mapsto> 3]\<rangle> \<longrightarrow>\<^sub>1  \<langle>?c; ?w, s[x \<mapsto> 3]\<rangle>" by simp
+  also have "\<langle>?c; ?w, s[x \<mapsto> 3]\<rangle> \<longrightarrow>\<^sub>1 \<langle>?w, s[x \<mapsto> 4]\<rangle>" by (rule Semi1, simp)
+  also have "\<langle>?w, s[x \<mapsto> 4]\<rangle> \<longrightarrow>\<^sub>1 \<langle>?if, s[x \<mapsto> 4]\<rangle>" ..
+  also have "\<langle>?if, s[x \<mapsto> 4]\<rangle> \<longrightarrow>\<^sub>1  \<langle>?c; ?w, s[x \<mapsto> 4]\<rangle>" by simp
+  also have "\<langle>?c; ?w, s[x \<mapsto> 4]\<rangle> \<longrightarrow>\<^sub>1 \<langle>?w, s[x \<mapsto> 5]\<rangle>" by (rule Semi1, simp) 
+  oops
+
+subsection "Basic properties"
+
+text {* 
+  There are no \emph{stuck} programs:
+*}
+lemma no_stuck: "\<exists>y. \<langle>c,s\<rangle> \<longrightarrow>\<^sub>1 y"
+proof (induct c)
+  -- "case Semi:"
+  fix c1 c2 assume "\<exists>y. \<langle>c1,s\<rangle> \<longrightarrow>\<^sub>1 y" 
+  then obtain y where "\<langle>c1,s\<rangle> \<longrightarrow>\<^sub>1 y" ..
+  then obtain c1' s' where "\<langle>c1,s\<rangle> \<longrightarrow>\<^sub>1 \<langle>s'\<rangle> \<or> \<langle>c1,s\<rangle> \<longrightarrow>\<^sub>1 \<langle>c1',s'\<rangle>"
+    by (cases y, cases "fst y", auto)
+  thus "\<exists>s'. \<langle>c1;c2,s\<rangle> \<longrightarrow>\<^sub>1 s'" by auto
+next
+  -- "case If:"
+  fix b c1 c2 assume "\<exists>y. \<langle>c1,s\<rangle> \<longrightarrow>\<^sub>1 y" and "\<exists>y. \<langle>c2,s\<rangle> \<longrightarrow>\<^sub>1 y"
+  thus "\<exists>y. \<langle>\<IF> b \<THEN> c1 \<ELSE> c2, s\<rangle> \<longrightarrow>\<^sub>1 y" by (cases "b s") auto
+qed auto -- "the rest is trivial"
+
+text {*
+  If a configuration does not contain a statement, the program
+  has terminated and there is no next configuration:
+*}
+lemma stuck [dest]: "(None, s) \<longrightarrow>\<^sub>1 y \<Longrightarrow> False" by (auto elim: evalc1.elims)
+
+(*<*)
+(* fixme: relpow.simps don't work *)
+lemma rel_pow_0 [simp]: "!!R::('a*'a) set. R^0 = Id" by simp
+lemma rel_pow_Suc_0 [simp]: "!!R::('a*'a) set. R^(Suc 0) = R" by simp 
+lemmas [simp del] = relpow.simps
+(*>*)
+
+lemma evalc_None_0 [simp]: "\<langle>s\<rangle> -n\<rightarrow>\<^sub>1 y = (n = 0 \<and> y = \<langle>s\<rangle>)"
+  by (cases n) auto
+
+lemma SKIP_n: "\<langle>\<SKIP>, s\<rangle> -n\<rightarrow>\<^sub>1 \<langle>s'\<rangle> \<Longrightarrow> s' = s \<and> n=1" 
+  by (cases n) auto
+
+subsection "Equivalence to natural semantics (after Nielson and Nielson)"
+
+text {*
+  We first need two lemmas about semicolon statements:
+  decomposition and composition.
+*}
+lemma semiD:
+  "\<And>c1 c2 s s''. \<langle>c1; c2, s\<rangle> -n\<rightarrow>\<^sub>1 \<langle>s''\<rangle> \<Longrightarrow> 
+  \<exists>i j s'. \<langle>c1, s\<rangle> -i\<rightarrow>\<^sub>1 \<langle>s'\<rangle> \<and> \<langle>c2, s'\<rangle> -j\<rightarrow>\<^sub>1 \<langle>s''\<rangle> \<and> n = i+j"
+  (is "PROP ?P n")
+proof (induct n)
+  show "PROP ?P 0" by simp
+next
+  fix n assume IH: "PROP ?P n"
+  show "PROP ?P (Suc n)"
+  proof -
+    fix c1 c2 s s''
+    assume "\<langle>c1; c2, s\<rangle> -Suc n\<rightarrow>\<^sub>1 \<langle>s''\<rangle>"
+    then obtain y where
+      1: "\<langle>c1; c2, s\<rangle> \<longrightarrow>\<^sub>1 y" and
+      n: "y -n\<rightarrow>\<^sub>1 \<langle>s''\<rangle>"
+      by blast
+
+    from 1
+    show "\<exists>i j s'. \<langle>c1, s\<rangle> -i\<rightarrow>\<^sub>1 \<langle>s'\<rangle> \<and> \<langle>c2, s'\<rangle> -j\<rightarrow>\<^sub>1 \<langle>s''\<rangle> \<and> Suc n = i+j"
+      (is "\<exists>i j s'. ?Q i j s'")
+    proof (cases set: evalc1)
+      case Semi1
+      then obtain s' where
+        "y = \<langle>c2, s'\<rangle>" and "\<langle>c1, s\<rangle> \<longrightarrow>\<^sub>1 \<langle>s'\<rangle>"
+        by auto
+      with 1 n have "?Q 1 n s'" by simp
+      thus ?thesis by blast
+    next
+      case Semi2
+      then obtain c1' s' where
+        y:  "y = \<langle>c1'; c2, s'\<rangle>" and
+        c1: "\<langle>c1, s\<rangle> \<longrightarrow>\<^sub>1 \<langle>c1', s'\<rangle>"
+        by auto
+      with n have "\<langle>c1'; c2, s'\<rangle> -n\<rightarrow>\<^sub>1 \<langle>s''\<rangle>" by simp 
+      with IH obtain i j s0 where 
+        c1': "\<langle>c1',s'\<rangle> -i\<rightarrow>\<^sub>1 \<langle>s0\<rangle>" and
+        c2:  "\<langle>c2,s0\<rangle> -j\<rightarrow>\<^sub>1 \<langle>s''\<rangle>" and
+        i:   "n = i+j"
+        by blast
+          
+      from c1 c1'
+      have "\<langle>c1,s\<rangle> -(i+1)\<rightarrow>\<^sub>1 \<langle>s0\<rangle>" by (auto simp del: relpow.simps intro: rel_pow_Suc_I2)
+      with c2 i
+      have "?Q (i+1) j s0" by simp
+      thus ?thesis by blast
+    qed auto -- "the remaining cases cannot occur"
+  qed
+qed
+
+
+lemma semiI: 
+  "\<And>c0 s s''. \<langle>c0,s\<rangle> -n\<rightarrow>\<^sub>1 \<langle>s''\<rangle> \<Longrightarrow> \<langle>c1,s''\<rangle> \<longrightarrow>\<^sub>1\<^sup>* \<langle>s'\<rangle> \<Longrightarrow> \<langle>c0; c1, s\<rangle> \<longrightarrow>\<^sub>1\<^sup>* \<langle>s'\<rangle>"
+proof (induct n)
+  fix c0 s s'' assume "\<langle>c0,s\<rangle> -(0::nat)\<rightarrow>\<^sub>1 \<langle>s''\<rangle>"
+  hence False by simp
+  thus "?thesis c0 s s''" ..
+next
+  fix c0 s s'' n 
+  assume c0: "\<langle>c0,s\<rangle> -Suc n\<rightarrow>\<^sub>1 \<langle>s''\<rangle>"
+  assume c1: "\<langle>c1,s''\<rangle> \<longrightarrow>\<^sub>1\<^sup>* \<langle>s'\<rangle>"
+  assume IH: "\<And>c0 s s''.
+    \<langle>c0,s\<rangle> -n\<rightarrow>\<^sub>1 \<langle>s''\<rangle> \<Longrightarrow> \<langle>c1,s''\<rangle> \<longrightarrow>\<^sub>1\<^sup>* \<langle>s'\<rangle> \<Longrightarrow> \<langle>c0; c1,s\<rangle> \<longrightarrow>\<^sub>1\<^sup>* \<langle>s'\<rangle>"
+  from c0 obtain y where 
+    1: "\<langle>c0,s\<rangle> \<longrightarrow>\<^sub>1 y" and n: "y -n\<rightarrow>\<^sub>1 \<langle>s''\<rangle>" by blast
+  from 1 obtain c0' s0' where
+    "y = \<langle>s0'\<rangle> \<or> y = \<langle>c0', s0'\<rangle>" 
+    by (cases y, cases "fst y", auto)
+  moreover
+  { assume y: "y = \<langle>s0'\<rangle>"
+    with n have "s'' = s0'" by simp
+    with y 1 have "\<langle>c0; c1,s\<rangle> \<longrightarrow>\<^sub>1 \<langle>c1, s''\<rangle>" by blast
+    with c1 have "\<langle>c0; c1,s\<rangle> \<longrightarrow>\<^sub>1\<^sup>* \<langle>s'\<rangle>" by (blast intro: rtrancl_trans)
+  }
+  moreover
+  { assume y: "y = \<langle>c0', s0'\<rangle>"
+    with n have "\<langle>c0', s0'\<rangle> -n\<rightarrow>\<^sub>1 \<langle>s''\<rangle>" by blast
+    with IH c1 have "\<langle>c0'; c1,s0'\<rangle> \<longrightarrow>\<^sub>1\<^sup>* \<langle>s'\<rangle>" by blast
+    moreover
+    from y 1 have "\<langle>c0; c1,s\<rangle> \<longrightarrow>\<^sub>1 \<langle>c0'; c1,s0'\<rangle>" by blast
+    hence "\<langle>c0; c1,s\<rangle> \<longrightarrow>\<^sub>1\<^sup>* \<langle>c0'; c1,s0'\<rangle>" by blast
+    ultimately
+    have "\<langle>c0; c1,s\<rangle> \<longrightarrow>\<^sub>1\<^sup>* \<langle>s'\<rangle>" by (blast intro: rtrancl_trans)
+  }
+  ultimately
+  show "\<langle>c0; c1,s\<rangle> \<longrightarrow>\<^sub>1\<^sup>* \<langle>s'\<rangle>" by blast
+qed
+
+text {*
+  The easy direction of the equivalence proof:
+*}
+lemma evalc_imp_evalc1: 
+  "\<langle>c,s\<rangle> \<longrightarrow>\<^sub>c s' \<Longrightarrow> \<langle>c, s\<rangle> \<longrightarrow>\<^sub>1\<^sup>* \<langle>s'\<rangle>"
+proof -
+  assume "\<langle>c,s\<rangle> \<longrightarrow>\<^sub>c s'"
+  thus "\<langle>c, s\<rangle> \<longrightarrow>\<^sub>1\<^sup>* \<langle>s'\<rangle>"
+  proof induct
+    fix s show "\<langle>\<SKIP>,s\<rangle> \<longrightarrow>\<^sub>1\<^sup>* \<langle>s\<rangle>" by auto
+  next
+    fix x a s show "\<langle>x :== a ,s\<rangle> \<longrightarrow>\<^sub>1\<^sup>* \<langle>s[x\<mapsto>a s]\<rangle>" by auto
+  next
+    fix c0 c1 s s'' s'
+    assume "\<langle>c0,s\<rangle> \<longrightarrow>\<^sub>1\<^sup>* \<langle>s''\<rangle>"
+    then obtain n where "\<langle>c0,s\<rangle> -n\<rightarrow>\<^sub>1 \<langle>s''\<rangle>" by (blast dest: rtrancl_imp_rel_pow)
+    moreover
+    assume "\<langle>c1,s''\<rangle> \<longrightarrow>\<^sub>1\<^sup>* \<langle>s'\<rangle>"
+    ultimately
+    show "\<langle>c0; c1,s\<rangle> \<longrightarrow>\<^sub>1\<^sup>* \<langle>s'\<rangle>" by (rule semiI)
+  next
+    fix s::state and b c0 c1 s'
+    assume "b s"
+    hence "\<langle>\<IF> b \<THEN> c0 \<ELSE> c1,s\<rangle> \<longrightarrow>\<^sub>1 \<langle>c0,s\<rangle>" by simp
+    also assume "\<langle>c0,s\<rangle> \<longrightarrow>\<^sub>1\<^sup>* \<langle>s'\<rangle>" 
+    finally show "\<langle>\<IF> b \<THEN> c0 \<ELSE> c1,s\<rangle> \<longrightarrow>\<^sub>1\<^sup>* \<langle>s'\<rangle>" .
+  next
+    fix s::state and b c0 c1 s'
+    assume "\<not>b s"
+    hence "\<langle>\<IF> b \<THEN> c0 \<ELSE> c1,s\<rangle> \<longrightarrow>\<^sub>1 \<langle>c1,s\<rangle>" by simp
+    also assume "\<langle>c1,s\<rangle> \<longrightarrow>\<^sub>1\<^sup>* \<langle>s'\<rangle>"
+    finally show "\<langle>\<IF> b \<THEN> c0 \<ELSE> c1,s\<rangle> \<longrightarrow>\<^sub>1\<^sup>* \<langle>s'\<rangle>" .
+  next
+    fix b c and s::state
+    assume b: "\<not>b s"
+    let ?if = "\<IF> b \<THEN> c; \<WHILE> b \<DO> c \<ELSE> \<SKIP>"
+    have "\<langle>\<WHILE> b \<DO> c,s\<rangle> \<longrightarrow>\<^sub>1 \<langle>?if, s\<rangle>" by blast
+    also have "\<langle>?if,s\<rangle> \<longrightarrow>\<^sub>1 \<langle>\<SKIP>, s\<rangle>" by (simp add: b)
+    also have "\<langle>\<SKIP>, s\<rangle> \<longrightarrow>\<^sub>1 \<langle>s\<rangle>" by blast
+    finally show "\<langle>\<WHILE> b \<DO> c,s\<rangle> \<longrightarrow>\<^sub>1\<^sup>* \<langle>s\<rangle>" ..
+  next
+    fix b c s s'' s'
+    let ?w  = "\<WHILE> b \<DO> c"
+    let ?if = "\<IF> b \<THEN> c; ?w \<ELSE> \<SKIP>"
+    assume w: "\<langle>?w,s''\<rangle> \<longrightarrow>\<^sub>1\<^sup>* \<langle>s'\<rangle>"
+    assume c: "\<langle>c,s\<rangle> \<longrightarrow>\<^sub>1\<^sup>* \<langle>s''\<rangle>"
+    assume b: "b s"
+    have "\<langle>?w,s\<rangle> \<longrightarrow>\<^sub>1 \<langle>?if, s\<rangle>" by blast
+    also have "\<langle>?if, s\<rangle> \<longrightarrow>\<^sub>1 \<langle>c; ?w, s\<rangle>" by (simp add: b)
+    also 
+    from c obtain n where "\<langle>c,s\<rangle> -n\<rightarrow>\<^sub>1 \<langle>s''\<rangle>" by (blast dest: rtrancl_imp_rel_pow)
+    with w have "\<langle>c; ?w,s\<rangle> \<longrightarrow>\<^sub>1\<^sup>* \<langle>s'\<rangle>" by - (rule semiI)
+    finally show "\<langle>\<WHILE> b \<DO> c,s\<rangle> \<longrightarrow>\<^sub>1\<^sup>* \<langle>s'\<rangle>" ..
+  qed
+qed
+
+text {*
+  Finally, the equivalence theorem:
+*}
+theorem evalc_equiv_evalc1:
+  "\<langle>c, s\<rangle> \<longrightarrow>\<^sub>c s' = \<langle>c,s\<rangle> \<longrightarrow>\<^sub>1\<^sup>* \<langle>s'\<rangle>"
+proof
+  assume "\<langle>c,s\<rangle> \<longrightarrow>\<^sub>c s'"
+  show "\<langle>c, s\<rangle> \<longrightarrow>\<^sub>1\<^sup>* \<langle>s'\<rangle>" by (rule evalc_imp_evalc1)
+next  
+  assume "\<langle>c, s\<rangle> \<longrightarrow>\<^sub>1\<^sup>* \<langle>s'\<rangle>"
+  then obtain n where "\<langle>c, s\<rangle> -n\<rightarrow>\<^sub>1 \<langle>s'\<rangle>" by (blast dest: rtrancl_imp_rel_pow)
+  moreover
+  have "\<And>c s s'. \<langle>c, s\<rangle> -n\<rightarrow>\<^sub>1 \<langle>s'\<rangle> \<Longrightarrow> \<langle>c,s\<rangle> \<longrightarrow>\<^sub>c s'" 
+  proof (induct rule: nat_less_induct)
+    fix n
+    assume IH: "\<forall>m. m < n \<longrightarrow> (\<forall>c s s'. \<langle>c, s\<rangle> -m\<rightarrow>\<^sub>1 \<langle>s'\<rangle> \<longrightarrow> \<langle>c,s\<rangle> \<longrightarrow>\<^sub>c s')"
+    fix c s s'
+    assume c:  "\<langle>c, s\<rangle> -n\<rightarrow>\<^sub>1 \<langle>s'\<rangle>"
+    then obtain m where n: "n = Suc m" by (cases n) auto
+    with c obtain y where 
+      c': "\<langle>c, s\<rangle> \<longrightarrow>\<^sub>1 y" and m: "y -m\<rightarrow>\<^sub>1 \<langle>s'\<rangle>" by blast
+    show "\<langle>c,s\<rangle> \<longrightarrow>\<^sub>c s'" 
+    proof (cases c)
+      case SKIP
+      with c n show ?thesis by auto
+    next 
+      case Assign
+      with c n show ?thesis by auto
+    next
+      fix c1 c2 assume semi: "c = (c1; c2)"
+      with c obtain i j s'' where
+        c1: "\<langle>c1, s\<rangle> -i\<rightarrow>\<^sub>1 \<langle>s''\<rangle>" and
+        c2: "\<langle>c2, s''\<rangle> -j\<rightarrow>\<^sub>1 \<langle>s'\<rangle>" and
+        ij: "n = i+j"
+        by (blast dest: semiD)
+      from c1 c2 obtain 
+        "0 < i" and "0 < j" by (cases i, auto, cases j, auto)
+      with ij obtain
+        i: "i < n" and j: "j < n" by simp
+      from c1 i IH
+      have "\<langle>c1,s\<rangle> \<longrightarrow>\<^sub>c s''" by blast
+      moreover
+      from c2 j IH
+      have "\<langle>c2,s''\<rangle> \<longrightarrow>\<^sub>c s'" by blast
+      moreover
+      note semi
+      ultimately
+      show "\<langle>c,s\<rangle> \<longrightarrow>\<^sub>c s'" by blast
+    next
+      fix b c1 c2 assume If: "c = \<IF> b \<THEN> c1 \<ELSE> c2"
+      { assume True: "b s = True"
+        with If c n
+        have "\<langle>c1,s\<rangle> -m\<rightarrow>\<^sub>1 \<langle>s'\<rangle>" by auto      
+        with n IH
+        have "\<langle>c1,s\<rangle> \<longrightarrow>\<^sub>c s'" by blast
+        with If True
+        have "\<langle>c,s\<rangle> \<longrightarrow>\<^sub>c s'" by simp        
+      }
+      moreover
+      { assume False: "b s = False"
+        with If c n
+        have "\<langle>c2,s\<rangle> -m\<rightarrow>\<^sub>1 \<langle>s'\<rangle>" by auto      
+        with n IH
+        have "\<langle>c2,s\<rangle> \<longrightarrow>\<^sub>c s'" by blast
+        with If False
+        have "\<langle>c,s\<rangle> \<longrightarrow>\<^sub>c s'" by simp        
+      }
+      ultimately
+      show "\<langle>c,s\<rangle> \<longrightarrow>\<^sub>c s'" by (cases "b s") auto
+    next
+      fix b c' assume w: "c = \<WHILE> b \<DO> c'"
+      with c n 
+      have "\<langle>\<IF> b \<THEN> c'; \<WHILE> b \<DO> c' \<ELSE> \<SKIP>,s\<rangle> -m\<rightarrow>\<^sub>1 \<langle>s'\<rangle>"
+        (is "\<langle>?if,_\<rangle> -m\<rightarrow>\<^sub>1 _") by auto
+      with n IH
+      have "\<langle>\<IF> b \<THEN> c'; \<WHILE> b \<DO> c' \<ELSE> \<SKIP>,s\<rangle> \<longrightarrow>\<^sub>c s'" by blast
+      moreover note unfold_while [of b c']
+      -- {* @{thm unfold_while [of b c']} *}
+      ultimately      
+      have "\<langle>\<WHILE> b \<DO> c',s\<rangle> \<longrightarrow>\<^sub>c s'" by (blast dest: equivD2)
+      with w show "\<langle>c,s\<rangle> \<longrightarrow>\<^sub>c s'" by simp
+    qed
+  qed
+  ultimately
+  show "\<langle>c,s\<rangle> \<longrightarrow>\<^sub>c s'" by blast
+qed
+
+
+subsection "Winskel's Proof"
+
+declare rel_pow_0_E [elim!]
+
+text {*
+  Winskel's small step rules are a bit different \cite{Winskel}; 
+  we introduce their equivalents as derived rules:
+*}
+lemma whileFalse1 [intro]:
+  "\<not> b s \<Longrightarrow> \<langle>\<WHILE> b \<DO> c,s\<rangle> \<longrightarrow>\<^sub>1\<^sup>* \<langle>s\<rangle>" (is "_ \<Longrightarrow> \<langle>?w, s\<rangle> \<longrightarrow>\<^sub>1\<^sup>* \<langle>s\<rangle>")  
+proof -
+  assume "\<not>b s"
+  have "\<langle>?w, s\<rangle> \<longrightarrow>\<^sub>1 \<langle>\<IF> b \<THEN> c;?w \<ELSE> \<SKIP>, s\<rangle>" ..
+  also have "\<langle>\<IF> b \<THEN> c;?w \<ELSE> \<SKIP>, s\<rangle> \<longrightarrow>\<^sub>1 \<langle>\<SKIP>, s\<rangle>" ..
+  also have "\<langle>\<SKIP>, s\<rangle> \<longrightarrow>\<^sub>1 \<langle>s\<rangle>" ..
+  finally show "\<langle>?w, s\<rangle> \<longrightarrow>\<^sub>1\<^sup>* \<langle>s\<rangle>" ..
+qed
+
+lemma whileTrue1 [intro]:
+  "b s \<Longrightarrow> \<langle>\<WHILE> b \<DO> c,s\<rangle> \<longrightarrow>\<^sub>1\<^sup>* \<langle>c;\<WHILE> b \<DO> c, s\<rangle>" 
+  (is "_ \<Longrightarrow> \<langle>?w, s\<rangle> \<longrightarrow>\<^sub>1\<^sup>* \<langle>c;?w,s\<rangle>")
+proof -
+  assume "b s"
+  have "\<langle>?w, s\<rangle> \<longrightarrow>\<^sub>1 \<langle>\<IF> b \<THEN> c;?w \<ELSE> \<SKIP>, s\<rangle>" ..
+  also have "\<langle>\<IF> b \<THEN> c;?w \<ELSE> \<SKIP>, s\<rangle> \<longrightarrow>\<^sub>1 \<langle>c;?w, s\<rangle>" ..
+  finally show "\<langle>?w, s\<rangle> \<longrightarrow>\<^sub>1\<^sup>* \<langle>c;?w,s\<rangle>" ..
+qed
+
+inductive_cases evalc1_SEs: 
+  "\<langle>\<SKIP>,s\<rangle> \<longrightarrow>\<^sub>1 t" 
+  "\<langle>x:==a,s\<rangle> \<longrightarrow>\<^sub>1 t"
+  "\<langle>c1;c2, s\<rangle> \<longrightarrow>\<^sub>1 t"
+  "\<langle>\<IF> b \<THEN> c1 \<ELSE> c2, s\<rangle> \<longrightarrow>\<^sub>1 t"
+  "\<langle>\<WHILE> b \<DO> c, s\<rangle> \<longrightarrow>\<^sub>1 t"
+
+inductive_cases evalc1_E: "\<langle>\<WHILE> b \<DO> c, s\<rangle> \<longrightarrow>\<^sub>1 t"
+
+declare evalc1_SEs [elim!]
+
+lemma evalc_impl_evalc1: "\<langle>c,s\<rangle> \<longrightarrow>\<^sub>c s1 \<Longrightarrow> \<langle>c,s\<rangle> \<longrightarrow>\<^sub>1\<^sup>* \<langle>s1\<rangle>"
+apply (erule evalc.induct)
+
+-- SKIP 
+apply blast
+
+-- ASSIGN 
+apply fast
+
+-- SEMI 
+apply (fast dest: rtrancl_imp_UN_rel_pow intro: semiI)
+
+-- IF 
+apply (fast intro: rtrancl_into_rtrancl2)
+apply (fast intro: rtrancl_into_rtrancl2)
+
+-- WHILE 
+apply fast
+apply (fast dest: rtrancl_imp_UN_rel_pow intro: rtrancl_into_rtrancl2 semiI)
+
+done
+
+
+lemma lemma2 [rule_format (no_asm)]: 
+  "\<forall>c d s u. \<langle>c;d,s\<rangle> -n\<rightarrow>\<^sub>1 \<langle>u\<rangle> \<longrightarrow> (\<exists>t m. \<langle>c,s\<rangle> \<longrightarrow>\<^sub>1\<^sup>* \<langle>t\<rangle> \<and> \<langle>d,t\<rangle> -m\<rightarrow>\<^sub>1 \<langle>u\<rangle> \<and> m \<le> n)"
+apply (induct_tac "n")
+ -- "case n = 0"
+ apply fastsimp
+-- "induction step"
+apply (fast intro!: le_SucI le_refl dest!: rel_pow_Suc_D2 
+            elim!: rel_pow_imp_rtrancl rtrancl_into_rtrancl2)
+done
+
+lemma evalc1_impl_evalc [rule_format (no_asm)]: 
+  "\<forall>s t. \<langle>c,s\<rangle> \<longrightarrow>\<^sub>1\<^sup>* \<langle>t\<rangle> \<longrightarrow> \<langle>c,s\<rangle> \<longrightarrow>\<^sub>c t"
+apply (induct_tac "c")
+apply (safe dest!: rtrancl_imp_UN_rel_pow)
+
+-- SKIP
+apply (simp add: SKIP_n)
+
+-- ASSIGN 
+apply (fastsimp elim: rel_pow_E2)
+
+-- SEMI
+apply (fast dest!: rel_pow_imp_rtrancl lemma2)
+
+-- IF 
+apply (erule rel_pow_E2)
+apply simp
+apply (fast dest!: rel_pow_imp_rtrancl)
+
+-- "WHILE, induction on the length of the computation"
+apply (rename_tac b c s t n)
+apply (erule_tac P = "?X -n\<rightarrow>\<^sub>1 ?Y" in rev_mp)
+apply (rule_tac x = "s" in spec)
+apply (induct_tac "n" rule: nat_less_induct)
+apply (intro strip)
+apply (erule rel_pow_E2)
+ apply simp
+apply (erule evalc1_E)
+
+apply simp
+apply (case_tac "b x")
+ -- WhileTrue
+ apply (erule rel_pow_E2)
+  apply simp
+ apply (clarify dest!: lemma2)
+ apply (erule allE, erule allE, erule impE, assumption)
+ apply (erule_tac x=mb in allE, erule impE, fastsimp)
+ apply blast
+-- WhileFalse 
+apply (erule rel_pow_E2)
+ apply simp
+apply (simp add: SKIP_n)
+done
+
+
+text {* proof of the equivalence of evalc and evalc1 *}
+lemma evalc1_eq_evalc: "(\<langle>c, s\<rangle> \<longrightarrow>\<^sub>1\<^sup>* \<langle>t\<rangle>) = (\<langle>c,s\<rangle> \<longrightarrow>\<^sub>c t)"
+apply (fast elim!: evalc1_impl_evalc evalc_impl_evalc1)
+done
+
+
+subsection "A proof without n"
+
+text {*
+  The inductions are a bit awkward to write in this section,
+  because @{text None} as result statement in the small step
+  semantics doesn't have a direct counterpart in the big step
+  semantics. 
+
+  Winskel's small step rule set (using the @{text "\<SKIP>"} statement
+  to indicate termination) is better suited for this proof.
+*}
+
+lemma my_lemma1 [rule_format (no_asm)]: 
+  "\<langle>c1,s1\<rangle> \<longrightarrow>\<^sub>1\<^sup>* \<langle>s2\<rangle> \<Longrightarrow> \<langle>c2,s2\<rangle> \<longrightarrow>\<^sub>1\<^sup>* cs3 \<Longrightarrow> \<langle>c1;c2,s1\<rangle> \<longrightarrow>\<^sub>1\<^sup>* cs3"
+proof -
+  -- {* The induction rule needs @{text P} to be a function of @{term "Some c1"} *}
+  have "\<langle>c1,s1\<rangle> \<longrightarrow>\<^sub>1\<^sup>* \<langle>s2\<rangle> \<Longrightarrow> \<langle>c2,s2\<rangle> \<longrightarrow>\<^sub>1\<^sup>* cs3 \<longrightarrow> 
+       \<langle>(\<lambda>c. if c = None then c2 else the c; c2) (Some c1),s1\<rangle> \<longrightarrow>\<^sub>1\<^sup>* cs3"
+    apply (erule converse_rtrancl_induct2)
+     apply simp
+    apply (rename_tac c s')
+    apply simp
+    apply (rule conjI)
+     apply (fast dest: stuck)
+    apply clarify
+    apply (case_tac c)
+    apply (auto intro: rtrancl_into_rtrancl2)
+    done
+  moreover assume "\<langle>c1,s1\<rangle> \<longrightarrow>\<^sub>1\<^sup>* \<langle>s2\<rangle>" "\<langle>c2,s2\<rangle> \<longrightarrow>\<^sub>1\<^sup>* cs3"
+  ultimately show "\<langle>c1;c2,s1\<rangle> \<longrightarrow>\<^sub>1\<^sup>* cs3" by simp
+qed
+
+lemma evalc_impl_evalc1: "\<langle>c,s\<rangle> \<longrightarrow>\<^sub>c s1 \<Longrightarrow> \<langle>c,s\<rangle> \<longrightarrow>\<^sub>1\<^sup>* \<langle>s1\<rangle>"
+apply (erule evalc.induct)
+
+-- SKIP 
+apply fast
+
+-- ASSIGN
+apply fast
+
+-- SEMI 
+apply (fast intro: my_lemma1)
+
+-- IF
+apply (fast intro: rtrancl_into_rtrancl2)
+apply (fast intro: rtrancl_into_rtrancl2) 
+
+-- WHILE 
+apply fast
+apply (fast intro: rtrancl_into_rtrancl2 my_lemma1)
+
+done
+
+text {*
+  The opposite direction is based on a Coq proof done by Ranan Fraer and
+  Yves Bertot. The following sketch is from an email by Ranan Fraer.
+
+\begin{verbatim}
+First we've broke it into 2 lemmas:
+
+Lemma 1
+((c,s) --> (SKIP,t)) => (<c,s> -c-> t)
+
+This is a quick one, dealing with the cases skip, assignment
+and while_false.
+
+Lemma 2
+((c,s) -*-> (c',s')) /\ <c',s'> -c'-> t
+  => 
+<c,s> -c-> t
+
+This is proved by rule induction on the  -*-> relation
+and the induction step makes use of a third lemma: 
+
+Lemma 3
+((c,s) --> (c',s')) /\ <c',s'> -c'-> t
+  => 
+<c,s> -c-> t
+
+This captures the essence of the proof, as it shows that <c',s'> 
+behaves as the continuation of <c,s> with respect to the natural
+semantics.
+The proof of Lemma 3 goes by rule induction on the --> relation,
+dealing with the cases sequence1, sequence2, if_true, if_false and
+while_true. In particular in the case (sequence1) we make use again
+of Lemma 1.
+\end{verbatim}
+*}
+
+inductive_cases evalc1_term_cases: "\<langle>c,s\<rangle> \<longrightarrow>\<^sub>1 \<langle>s'\<rangle>"
+
+lemma FB_lemma3 [rule_format]:
+  "(c,s) \<longrightarrow>\<^sub>1 (c',s') \<Longrightarrow> c \<noteq> None \<longrightarrow>
+  (\<forall>t. \<langle>if c'=None then \<SKIP> else the c',s'\<rangle> \<longrightarrow>\<^sub>c t \<longrightarrow> \<langle>the c,s\<rangle> \<longrightarrow>\<^sub>c t)"
+  apply (erule evalc1.induct)
+  apply (auto elim!: evalc1_term_cases equivD2 [OF unfold_while])
+  done
+
+lemma rtrancl_stuck: "\<langle>s\<rangle> \<longrightarrow>\<^sub>1\<^sup>* s' \<Longrightarrow> s' = (None, s)"
+  by (erule rtrancl_induct) (auto dest: stuck)
+
+lemma FB_lemma2 [rule_format]:
+  "(c,s) \<longrightarrow>\<^sub>1\<^sup>* (c',s') \<Longrightarrow> c \<noteq> None \<longrightarrow> 
+   \<langle>if c' = None then \<SKIP> else the c',s'\<rangle> \<longrightarrow>\<^sub>c t \<longrightarrow> \<langle>the c,s\<rangle> \<longrightarrow>\<^sub>c t" 
+  apply (erule converse_rtrancl_induct2)
+   apply simp
+  apply clarsimp
+  apply (fastsimp elim!: evalc1_term_cases dest: rtrancl_stuck intro: FB_lemma3)
+  done
+
+lemma evalc1_impl_evalc: "\<langle>c,s\<rangle> \<longrightarrow>\<^sub>1\<^sup>* \<langle>t\<rangle> \<Longrightarrow> \<langle>c,s\<rangle> \<longrightarrow>\<^sub>c t"
+  apply (fastsimp dest: FB_lemma2)
+  done
 
 end
