src/HOL/IMP/Denotation.thy
@@ -2,28 +2,79 @@
     ID:         $Id$
     Author:     Heiko Loetzbeyer & Robert Sandner, TUM
     Copyright   1994 TUM
-
-Denotational semantics of commands
 *)
 
-Denotation = Natural + 
+header "Denotational Semantics of Commands"
 
-types com_den = "(state*state)set"
+theory Denotation = Natural:
+
+types com_den = "(state\<times>state)set"
 
 constdefs
-  Gamma :: [bexp,com_den] => (com_den => com_den)
-           "Gamma b cd == (%phi.{(s,t). (s,t) : (phi O cd) & b(s)} Un 
-                                 {(s,t). s=t & ~b(s)})"
+  Gamma :: "[bexp,com_den] => (com_den => com_den)"
+  "Gamma b cd == (\<lambda>phi. {(s,t). (s,t) \<in> (phi O cd) \<and> b s} \<union> 
+                        {(s,t). s=t \<and> \<not>b s})"
     
 consts
-  C     :: com => com_den
+  C :: "com => com_den"
 
 primrec
-  C_skip    "C(SKIP) = Id"
-  C_assign  "C(x :== a) = {(s,t). t = s[x::=a(s)]}"
-  C_comp    "C(c0 ; c1) = C(c1) O C(c0)"
-  C_if      "C(IF b THEN c1 ELSE c2) = {(s,t). (s,t) : C(c1) & b(s)} Un
-                                       {(s,t). (s,t) : C(c2) & ~ b(s)}"
-  C_while   "C(WHILE b DO c) = lfp (Gamma b (C c))"
+  C_skip:   "C \<SKIP>   = Id"
+  C_assign: "C (x :== a) = {(s,t). t = s[x\<mapsto>a(s)]}"
+  C_comp:   "C (c0;c1)   = C(c1) O C(c0)"
+  C_if:     "C (\<IF> b \<THEN> c1 \<ELSE> c2) = {(s,t). (s,t) \<in> C c1 \<and> b s} \<union>
+                                                 {(s,t). (s,t) \<in> C c2 \<and> \<not>b s}"
+  C_while:  "C(\<WHILE> b \<DO> c) = lfp (Gamma b (C c))"
+
+
+(**** mono (Gamma(b,c)) ****)
+
+lemma Gamma_mono: "mono (Gamma b c)"
+  by (unfold Gamma_def mono_def) fast
+
+lemma C_While_If: "C(\<WHILE> b \<DO> c) = C(\<IF> b \<THEN> c;\<WHILE> b \<DO> c \<ELSE> \<SKIP>)"
+apply (simp (no_asm))
+apply (subst lfp_unfold [OF Gamma_mono],
+       subst Gamma_def [THEN meta_eq_to_obj_eq, THEN fun_cong],
+       simp)
+done
+
+(* Operational Semantics implies Denotational Semantics *)
+
+lemma com1: "\<langle>c,s\<rangle> \<longrightarrow>\<^sub>c t \<Longrightarrow> (s,t) \<in> C(c)"
+
+(* start with rule induction *)
+apply (erule evalc.induct)
+apply auto
+(* while *)
+apply (unfold Gamma_def)
+apply (subst lfp_unfold[OF Gamma_mono, simplified Gamma_def])
+apply fast
+apply (subst lfp_unfold[OF Gamma_mono, simplified Gamma_def])
+apply fast
+done
+
+(* Denotational Semantics implies Operational Semantics *)
+
+lemma com2 [rule_format]: "\<forall>s t. (s,t)\<in>C(c) \<longrightarrow> \<langle>c,s\<rangle> \<longrightarrow>\<^sub>c t"
+apply (induct_tac "c")
+
+apply (simp_all (no_asm_use))
+apply fast
+apply fast
+
+(* while *)
+apply (intro strip)
+apply (erule lfp_induct [OF _ Gamma_mono])
+apply (unfold Gamma_def)
+apply fast
+done
+
+
+(**** Proof of Equivalence ****)
+
+lemma denotational_is_natural: "(s,t) \<in> C(c)  =  (\<langle>c,s\<rangle> \<longrightarrow>\<^sub>c t)"
+apply (fast elim: com2 dest: com1)
+done
 
 end
