src/HOL/IMP/Examples.thy
@@ -4,17 +4,83 @@
     Copyright   2000 TUM
 *)
 
-Examples = Natural +
+header "Examples"
 
-defs (* bring up the deferred definition for update *)
+theory Examples = Natural:
 
- update_def "update == fun_upd"
+constdefs  
+  factorial :: "loc => loc => com"
+  "factorial a b == b :== (%s. 1);
+                    \<WHILE> (%s. s a ~= 0) \<DO>
+                    (b :== (%s. s b * s a); a :== (%s. s a - 1))"
 
-constdefs
-  
-  factorial :: loc => loc => com
- "factorial a b == b :== (%s. 1);
-               WHILE (%s. s a ~= 0) DO
-                 (b :== (%s. s b * s a); a :== (%s. s a - 1))"
+declare update_def [simp]
+
+subsection "An example due to Tony Hoare"
+
+lemma lemma1 [rule_format (no_asm)]: 
+  "[| !x. P x \<longrightarrow> Q x; \<langle>w,s\<rangle> \<longrightarrow>\<^sub>c t |] ==>
+  !c. w = While P c \<longrightarrow> \<langle>While Q c,t\<rangle> \<longrightarrow>\<^sub>c u \<longrightarrow> \<langle>While Q c,s\<rangle> \<longrightarrow>\<^sub>c u"
+apply (erule evalc.induct)
+apply auto
+done
+
+
+lemma lemma2 [rule_format (no_asm)]: 
+  "[| !x. P x \<longrightarrow> Q x; \<langle>w,s\<rangle> \<longrightarrow>\<^sub>c u |] ==>  
+  !c. w = While Q c \<longrightarrow> \<langle>While P c; While Q c,s\<rangle> \<longrightarrow>\<^sub>c u"
+apply (erule evalc.induct)
+apply (simp_all (no_asm_simp))
+apply blast
+apply (case_tac "P s")
+apply auto
+done
+
+
+lemma Hoare_example: "!x. P x \<longrightarrow> Q x ==>  
+  (\<langle>While P c; While Q c, s\<rangle> \<longrightarrow>\<^sub>c t) = (\<langle>While Q c, s\<rangle> \<longrightarrow>\<^sub>c t)"
+  by (blast intro: lemma1 lemma2 dest: semi [THEN iffD1])
+
+
+subsection "Factorial"
+
+lemma factorial_3: "a~=b ==>  
+  \<langle>factorial a b, Mem(a:=3)\<rangle> \<longrightarrow>\<^sub>c Mem(b:=6, a:=0)"
+apply (unfold factorial_def)
+apply simp
+done
+
+text {* the same in single step mode: *}
+lemmas [simp del] = evalc_cases
+lemma  "a~=b \<Longrightarrow> \<langle>factorial a b, Mem(a:=3)\<rangle> \<longrightarrow>\<^sub>c Mem(b:=6, a:=0)"
+apply (unfold factorial_def)
+apply (frule not_sym)
+apply (rule evalc.intros)
+apply  (rule evalc.intros)
+apply simp
+apply (rule evalc.intros)
+apply   simp
+apply  (rule evalc.intros)
+apply   (rule evalc.intros)
+apply  simp
+apply  (rule evalc.intros)
+apply simp
+apply (rule evalc.intros)
+apply   simp
+apply  (rule evalc.intros)
+apply   (rule evalc.intros)
+apply  simp
+apply  (rule evalc.intros)
+apply simp
+apply (rule evalc.intros)
+apply   simp
+apply  (rule evalc.intros)
+apply   (rule evalc.intros)
+apply  simp
+apply  (rule evalc.intros)
+apply simp
+apply (rule evalc.intros)
+apply simp
+done
   
 end
