src/HOL/IMP/VC.thy
@@ -8,7 +8,9 @@ vc:   verification-conditions
 awp:   weakest (liberal) precondition
 *)
 
-VC  =  Hoare +
+header "Verification Conditions"
+
+theory VC = Hoare:
 
 datatype  acom = Askip
                | Aass   loc aexp
@@ -17,45 +19,121 @@ datatype  acom = Askip
                | Awhile bexp assn acom
 
 consts
-  vc,awp :: acom => assn => assn
-  vcawp :: "acom => assn => assn * assn"
-  astrip :: acom => com
+  vc :: "acom => assn => assn"
+  awp :: "acom => assn => assn"
+  vcawp :: "acom => assn => assn \<times> assn"
+  astrip :: "acom => com"
 
 primrec
   "awp Askip Q = Q"
-  "awp (Aass x a) Q = (%s. Q(s[x::=a s]))"
+  "awp (Aass x a) Q = (\<lambda>s. Q(s[x\<mapsto>a s]))"
   "awp (Asemi c d) Q = awp c (awp d Q)"
-  "awp (Aif b c d) Q = (%s. (b s-->awp c Q s) & (~b s-->awp d Q s))" 
+  "awp (Aif b c d) Q = (\<lambda>s. (b s-->awp c Q s) & (~b s-->awp d Q s))" 
   "awp (Awhile b I c) Q = I"
 
 primrec
-  "vc Askip Q = (%s. True)"
-  "vc (Aass x a) Q = (%s. True)"
-  "vc (Asemi c d) Q = (%s. vc c (awp d Q) s & vc d Q s)"
-  "vc (Aif b c d) Q = (%s. vc c Q s & vc d Q s)" 
-  "vc (Awhile b I c) Q = (%s. (I s & ~b s --> Q s) &
+  "vc Askip Q = (\<lambda>s. True)"
+  "vc (Aass x a) Q = (\<lambda>s. True)"
+  "vc (Asemi c d) Q = (\<lambda>s. vc c (awp d Q) s & vc d Q s)"
+  "vc (Aif b c d) Q = (\<lambda>s. vc c Q s & vc d Q s)" 
+  "vc (Awhile b I c) Q = (\<lambda>s. (I s & ~b s --> Q s) &
                               (I s & b s --> awp c I s) & vc c I s)"
 
 primrec
   "astrip Askip = SKIP"
   "astrip (Aass x a) = (x:==a)"
   "astrip (Asemi c d) = (astrip c;astrip d)"
-  "astrip (Aif b c d) = (IF b THEN astrip c ELSE astrip d)"
-  "astrip (Awhile b I c) = (WHILE b DO astrip c)"
+  "astrip (Aif b c d) = (\<IF> b \<THEN> astrip c \<ELSE> astrip d)"
+  "astrip (Awhile b I c) = (\<WHILE> b \<DO> astrip c)"
 
 (* simultaneous computation of vc and awp: *)
 primrec
-  "vcawp Askip Q = (%s. True, Q)"
-  "vcawp (Aass x a) Q = (%s. True, %s. Q(s[x::=a s]))"
+  "vcawp Askip Q = (\<lambda>s. True, Q)"
+  "vcawp (Aass x a) Q = (\<lambda>s. True, \<lambda>s. Q(s[x\<mapsto>a s]))"
   "vcawp (Asemi c d) Q = (let (vcd,wpd) = vcawp d Q;
                               (vcc,wpc) = vcawp c wpd
-                          in (%s. vcc s & vcd s, wpc))"
+                          in (\<lambda>s. vcc s & vcd s, wpc))"
   "vcawp (Aif b c d) Q = (let (vcd,wpd) = vcawp d Q;
                               (vcc,wpc) = vcawp c Q
-                          in (%s. vcc s & vcd s,
-                              %s.(b s --> wpc s) & (~b s --> wpd s)))"
+                          in (\<lambda>s. vcc s & vcd s,
+                              \<lambda>s.(b s --> wpc s) & (~b s --> wpd s)))"
   "vcawp (Awhile b I c) Q = (let (vcc,wpc) = vcawp c I
-                             in (%s. (I s & ~b s --> Q s) &
+                             in (\<lambda>s. (I s & ~b s --> Q s) &
                                      (I s & b s --> wpc s) & vcc s, I))"
+
+(*
+Soundness and completeness of vc
+*)
+
+declare hoare.intros [intro]
+
+lemma l: "!s. P s --> P s" by fast
+
+lemma vc_sound: "!Q. (!s. vc c Q s) --> |- {awp c Q} astrip c {Q}"
+apply (induct_tac "c")
+    apply (simp_all (no_asm))
+    apply fast
+   apply fast
+  apply fast
+ (* if *)
+ apply (tactic "Deepen_tac 4 1")
+(* while *)
+apply (intro allI impI) 
+apply (rule conseq)
+  apply (rule l)
+ apply (rule While)
+ defer
+ apply fast
+apply (rule_tac P="awp acom fun2" in conseq)
+  apply fast
+ apply fast
+apply fast
+done
+
+lemma awp_mono [rule_format (no_asm)]: "!P Q. (!s. P s --> Q s) --> (!s. awp c P s --> awp c Q s)"
+apply (induct_tac "c")
+    apply (simp_all (no_asm_simp))
+apply (rule allI, rule allI, rule impI)
+apply (erule allE, erule allE, erule mp)
+apply (erule allE, erule allE, erule mp, assumption)
+done
+
+
+lemma vc_mono [rule_format (no_asm)]: "!P Q. (!s. P s --> Q s) --> (!s. vc c P s --> vc c Q s)"
+apply (induct_tac "c")
+    apply (simp_all (no_asm_simp))
+apply safe
+apply (erule allE,erule allE,erule impE,erule_tac [2] allE,erule_tac [2] mp) 
+prefer 2 apply assumption
+apply (fast elim: awp_mono)
+done
+
+lemma vc_complete: "|- {P}c{Q} ==>  
+   (? ac. astrip ac = c & (!s. vc ac Q s) & (!s. P s --> awp ac Q s))"
+apply (erule hoare.induct)
+     apply (rule_tac x = "Askip" in exI)
+     apply (simp (no_asm))
+    apply (rule_tac x = "Aass x a" in exI)
+    apply (simp (no_asm))
+   apply clarify
+   apply (rule_tac x = "Asemi ac aca" in exI)
+   apply (simp (no_asm_simp))
+   apply (fast elim!: awp_mono vc_mono)
+  apply clarify
+  apply (rule_tac x = "Aif b ac aca" in exI)
+  apply (simp (no_asm_simp))
+ apply clarify
+ apply (rule_tac x = "Awhile b P ac" in exI)
+ apply (simp (no_asm_simp))
+apply safe
+apply (rule_tac x = "ac" in exI)
+apply (simp (no_asm_simp))
+apply (fast elim!: awp_mono vc_mono)
+done
+
+lemma vcawp_vc_awp: "!Q. vcawp c Q = (vc c Q, awp c Q)"
+apply (induct_tac "c")
+apply (simp_all (no_asm_simp) add: Let_def)
+done
 
 end
