src/HOLCF/IMP/Denotational.thy
@@ -2,11 +2,13 @@
     ID:         $Id$
     Author:     Tobias Nipkow & Robert Sandner, TUM
     Copyright   1996 TUM
-
-Denotational semantics of commands in HOLCF
 *)
 
-Denotational = HOLCF + Natural +
+header "Denotational Semantics of Commands in HOLCF"
+
+theory Denotational = HOLCF + Natural:
+
+subsection "Definition"
 
 constdefs
    dlift :: "(('a::type) discr -> 'b::pcpo) => ('a lift -> 'b)"
@@ -15,13 +17,65 @@ constdefs
 consts D :: "com => state discr -> state lift"
 
 primrec
-  "D(SKIP) = (LAM s. Def(undiscr s))"
-  "D(X :== a) = (LAM s. Def((undiscr s)[X ::= a(undiscr s)]))"
+  "D(\<SKIP>) = (LAM s. Def(undiscr s))"
+  "D(X :== a) = (LAM s. Def((undiscr s)[X \<mapsto> a(undiscr s)]))"
   "D(c0 ; c1) = (dlift(D c1) oo (D c0))"
-  "D(IF b THEN c1 ELSE c2) =
+  "D(\<IF> b \<THEN> c1 \<ELSE> c2) =
 	(LAM s. if b(undiscr s) then (D c1)$s else (D c2)$s)"
-  "D(WHILE b DO c) =
+  "D(\<WHILE> b \<DO> c) =
 	fix$(LAM w s. if b(undiscr s) then (dlift w)$((D c)$s)
                       else Def(undiscr s))"
+
+subsection
+  "Equivalence of Denotational Semantics in HOLCF and Evaluation Semantics in HOL"
+
+lemma dlift_Def: "dlift f$(Def x) = f$(Discr x)"
+apply (unfold dlift_def)
+apply (simp (no_asm))
+done
+declare dlift_Def [simp]
+
+lemma cont_dlift: "cont(%f. dlift f)"
+apply (unfold dlift_def)
+apply (simp (no_asm))
+done
+declare cont_dlift [iff]
+
+lemma dlift_is_Def: 
+ "(dlift f$l = Def y) = (? x. l = Def x & f$(Discr x) = Def y)"
+apply (unfold dlift_def)
+apply (simp (no_asm) split add: lift.split)
+done
+declare dlift_is_Def [simp]
+
+lemma eval_implies_D [rule_format (no_asm)]: 
+  "\<langle>c,s\<rangle> \<longrightarrow>\<^sub>c t ==> D c$(Discr s) = (Def t)"
+apply (erule evalc.induct)
+      apply (simp_all (no_asm_simp))
+ apply (subst fix_eq)
+ apply simp
+apply (subst fix_eq)
+apply simp
+done
+
+lemma D_implies_eval [rule_format (no_asm)]: 
+  "!s t. D c$(Discr s) = (Def t) --> \<langle>c,s\<rangle> \<longrightarrow>\<^sub>c t"
+apply (induct_tac "c")
+    apply force
+   apply force
+  apply force
+ apply (simp (no_asm))
+ apply force
+apply (simp (no_asm))
+apply (rule fix_ind)
+  apply (fast intro!: adm_lemmas adm_chfindom ax_flat)
+ apply (simp (no_asm))
+apply (simp (no_asm))
+apply safe
+apply fast
+done
+
+lemma D_is_eval: "(D c$(Discr s) = (Def t)) = (\<langle>c,s\<rangle> \<longrightarrow>\<^sub>c t)"
+  by (fast elim!: D_implies_eval eval_implies_D)
 
 end
