src/HOLCF/IMP/HoareEx.thy
@@ -2,17 +2,32 @@
     ID:         $Id$
     Author:     Tobias Nipkow, TUM
     Copyright   1997 TUM
-
-An example from the HOLCF paper by Mueller, Nipkow, Oheimb, Slotosch.
-It demonstrates fixpoint reasoning by showing the correctness of the Hoare
-rule for while-loops.
 *)
 
-HoareEx = Denotational +
+header "Correctness of Hoare by Fixpoint Reasoning"
 
-types assn = state => bool
+theory HoareEx = Denotational:
 
-constdefs hoare_valid :: [assn,com,assn] => bool ("|= {(1_)}/ (_)/ {(1_)}" 50)
+text {*
+  An example from the HOLCF paper by Mueller, Nipkow, Oheimb, Slotosch \cite{MuellerNvOS99}.
+  It demonstrates fixpoint reasoning by showing the correctness of the Hoare
+  rule for while-loops.
+*}
+
+types assn = "state => bool"
+
+constdefs hoare_valid :: "[assn,com,assn] => bool" ("|= {(1_)}/ (_)/ {(1_)}" 50)
  "|= {A} c {B} == !s t. A s & D c $(Discr s) = Def t --> B t"
+
+lemma WHILE_rule_sound:
+  "|= {A} c {A} ==> |= {A} \<WHILE> b \<DO> c {%s. A s & ~b s}"
+  apply (unfold hoare_valid_def)
+  apply (simp (no_asm))
+  apply (rule fix_ind)
+    apply (simp (no_asm)) -- "simplifier with enhanced adm-tactic"
+   apply (simp (no_asm))
+  apply (simp (no_asm))
+  apply blast
+  done
 
 end
